Prove named PanStructs memory load conversion

scripts/hol-probes/pan_structs_mem_load_conversion_probeScript.sml
@@ -45,3 +45,37 @@ val _ = print_eval "mem_load_conversion_comb_multiword"
        SOME (convert_v ^comb_value),
      size_of_sh_with_ctxt [] (compile_shape [] ^comb_shape) =
        size_of_sh_with_ctxt [] ^comb_shape)``;
+
+val named_struct_ctxt =
+  ``[(strlit "Pair", <| fields := [(strlit "inner", Named (strlit "Inner"));
+                                   (strlit "last", One)]; size := 3 |>);
+     (strlit "Inner", <| fields := [(strlit "left", One);
+                                     (strlit "right", One)]; size := 2 |>)]``;
+val named_shape_ctxt =
+  ``MAP (λ(nm,info). (nm,info.fields)) ^named_struct_ctxt``;
+val named_shape = ``Named (strlit "Pair")``;
+val named_domain = ``{0w:8 word; 1w; 2w}``;
+val named_memory =
+  ``\a:8 word. if a = 0w then Word (7w:8 word)
+      else if a = 1w then Word (11w:8 word)
+      else if a = 2w then Word (13w:8 word)
+      else ARB``;
+val named_value =
+  ``NStruct (strlit "Pair")
+      [(strlit "inner", NStruct (strlit "Inner")
+        [(strlit "left", ValWord (7w:8 word));
+         (strlit "right", ValWord (11w:8 word))]);
+       (strlit "last", ValWord (13w:8 word))]``;
+val _ = print_eval "mem_load_conversion_named_nested"
+  ``(is_wf_shape (DROP 0 ^named_struct_ctxt) ^named_shape,
+     struct_infos_ok ^named_struct_ctxt,
+     mem_load ^named_shape 0w ^named_domain ^named_memory ^named_struct_ctxt =
+       SOME ^named_value,
+     mem_load (compile_shape_n ^named_shape_ctxt 0 ^named_shape) 0w
+       ^named_domain ^named_memory ^named_struct_ctxt =
+       SOME (convert_v ^named_value),
+     v_flds_ok ^named_struct_ctxt ^named_value,
+     size_of_sh_with_ctxt []
+       (compile_shape_n ^named_shape_ctxt 0 ^named_shape) =
+       size_of_sh_with_ctxt ^named_struct_ctxt ^named_shape)
+     ``;
